FormalVerifyMisc/FixedInt/Mod.lean
@@ -51,3 +51,67 @@ theorem int32_neg_mod (a b : Int32) (hlba : Int32.minValue < a) : (-a) % b = -(a
   rw [int32_toInt_neg (a % b) (int32_minval_lt_mod a b hlba)]
   rw [Int32.toInt_mod, Int32.toInt_mod]
   rw [int32_toInt_neg a hlba, Int.neg_tmod]
+
+-- I'm surprised this result doesn't already exist
+-- Gemini seems to think 'tmod_le_self' *does* exist,
+-- but I haven't been able to find it
+theorem int_tmod_le_self (m n : Int) (hmpos : 0 ≤ m) : m.tmod n ≤ m := by
+  by_cases h₀ : m < n
+  · rw [Int.tmod_eq_of_lt hmpos h₀]
+  by_cases h₁ : m < -n
+  · rw [← Int.tmod_neg]
+    rw [Int.tmod_eq_of_lt hmpos h₁]
+  by_cases hz : n = 0
+  · subst hz; simp
+  rename' hz => hnz; push_neg at hnz
+  apply le_of_lt
+  by_cases hnpos : 0 < n
+  · exact Int.lt_of_lt_of_le (Int.tmod_lt_of_pos m hnpos) (not_lt.mp h₀)
+  replace hnpos := Int.neg_pos.mpr (lt_of_le_of_ne (le_of_not_gt hnpos) hnz)
+  apply Int.lt_of_lt_of_le _ (not_lt.mp h₁)
+  rw [← Int.tmod_neg]
+  exact Int.tmod_lt_of_pos m hnpos
+
+lemma mul_tdiv_in_bounds_32_of_in_bounds_32
+  (m n : Int) (hmib : in_bounds_32 m) :
+  in_bounds_32 (n * (m.tdiv n)) := by
+  obtain ⟨lbm, ubm⟩ := hmib
+  have hrw : n * (m.tdiv n) = m - m.tmod n := by
+    apply eq_sub_of_add_eq
+    exact Int.mul_tdiv_add_tmod _ _
+  rw [hrw]; clear hrw
+  -- Handle the case where m = -2^31 so the remaining cases are symmetric
+  by_cases hmmv : m = -2^31
+  · subst hmmv
+    constructor <;> simp
+    · apply Int.tmod_nonneg; simp
+    · exact lt_of_le_of_lt (int_tmod_le_self _ n (by norm_num)) (by norm_num)
+  push_neg at hmmv
+  replace lbm := lt_of_le_of_ne lbm hmmv.symm; clear hmmv
+  apply in_bounds_32_of_abs_lt
+  -- Without loss of generality, m is non-negative
+  wlog h : 0 ≤ m
+  · rw [← Int.add_neg_eq_sub, ← Int.neg_tmod, ← abs_neg]
+    rw [Int.neg_add, Int.add_neg_eq_sub]
+    apply this (-m) n (neg_lt.mp lbm) (neg_lt_neg ubm)
+    exact neg_nonneg_of_nonpos (le_of_not_ge h)
+  apply abs_sub_lt_of_nonneg_of_lt h ubm (Int.tmod_nonneg _ h) (lt_of_le_of_lt _ ubm)
+  exact int_tmod_le_self _ _ h
+
+-- Prove when the defining equation for '%' holds for Int32
+theorem int32_mul_div_add_mod
+  (a b : Int32) (h : Int32.minValue < a ∨ b ≠ -1) : b * (a / b) + (a % b) = a := by
+  have := Int.mul_tdiv_add_tmod a.toInt b.toInt
+  have h₀ : in_bounds_32 (b.toInt * (a / b).toInt) := by
+    rw [int32_toInt_div a b h]
+    apply mul_tdiv_in_bounds_32_of_in_bounds_32
+    exact int32_in_bounds_toInt _
+  have h₁ : in_bounds_32 ((b * (a / b)).toInt + (a % b).toInt) := by
+    rw [int32_toInt_mul_of_bounds _ _ h₀]
+    rw [int32_toInt_div a b h, Int32.toInt_mod]
+    rw [this]
+    exact int32_in_bounds_toInt _
+  apply Int32.toInt_inj.mp
+  rw [int32_toInt_add_of_bounds _ _ h₁]
+  rw [int32_toInt_mul_of_bounds _ _ h₀]
+  rwa [Int32.toInt_mod, int32_toInt_div _ _ h]
